ProofForgeV2/Source/AstSpineDeclV1.lean
@@ -15,37 +15,37 @@ structure ConstDeclV1 where
   name : SourceNameComponentV1
   type_ : TypeV1
   value : ExprV1
-  deriving DecidableEq, Repr
+  deriving DecidableEq, Repr, Lean.ToExpr
 
 structure InvariantDeclV1 where
   name : SourceNameComponentV1
   predicate : ExprV1
-  deriving DecidableEq, Repr
+  deriving DecidableEq, Repr, Lean.ToExpr
 
 structure InitDeclV1 where
   params : Array ParamV1
   body : BlockV1
-  deriving DecidableEq, Repr
+  deriving DecidableEq, Repr, Lean.ToExpr
 
 structure EntryDeclV1 where
   name : SourceNameComponentV1
   params : Array ParamV1
   result : TypeV1
   body : BlockV1
-  deriving DecidableEq, Repr
+  deriving DecidableEq, Repr, Lean.ToExpr
 
 structure ViewDeclV1 where
   name : SourceNameComponentV1
   params : Array ParamV1
   result : TypeV1
   body : BlockV1
-  deriving DecidableEq, Repr
+  deriving DecidableEq, Repr, Lean.ToExpr
 
 structure FnDeclV1 where
   name : SourceNameComponentV1
   params : Array ParamV1
   result : TypeV1
   body : BlockV1
-  deriving DecidableEq, Repr
+  deriving DecidableEq, Repr, Lean.ToExpr
 
 end ProofForgeV2.Source.AstSpineDeclV1
